web-proof-machine/GadgetGameSolver/GadgetGameSolver/DFS.lean
@@ -221,53 +221,56 @@ elab stx:"#gadget_display" axioms?:("with_axioms")? name:str timeout?:(num)? : c
 
   logInfoAt stx m!"{proofLog}"
 
-  if timeout?.isNone && !tree.isClosed then
-    throwError "The proof tree is not closed."
-  let initDiagram := ProofResult.getGadgetGraph ⟨problemState.target, tree⟩
-  let initData : InitializationData := {
-    initialDiagram := initDiagram,
-    axioms := if axioms?.isSome then problemState.axioms else .empty
-  }
-  let jsonProps := Lean.toJson initData
-  Widget.savePanelWidgetInfo (hash GadgetGraph.javascript)
-    (return jsonProps) stx
+  -- if timeout?.isNone && !tree.isClosed then
+  --   throwError "The proof tree is not closed."
+  -- let initDiagram := ProofResult.getGadgetGraph ⟨problemState.target, tree⟩
+  -- let initData : InitializationData := {
+  --   initialDiagram := initDiagram,
+  --   axioms := if axioms?.isSome then problemState.axioms else .empty
+  -- }
+  -- let jsonProps := Lean.toJson initData
+  -- Widget.savePanelWidgetInfo (hash GadgetGraph.javascript)
+  --   (return jsonProps) stx
 
--- #gadget_display with_axioms "tim08"
+#gadget_display with_axioms "jovan02" 40
 
--- #exit
+#exit
 
--- #gadget_display with_axioms "tim_easy01" -- 6  - 5
--- #gadget_display with_axioms "tim_easy02" -- 40 - 29 | 32
--- #gadget_display with_axioms "tim_easy03" -- 40 - 11 - 13 - 5
--- #gadget_display with_axioms "tim_easy04" -- ∞  - 10 - 11
--- #gadget_display with_axioms "tim_easy05" -- ∞  - 59
--- #gadget_display with_axioms "tim_easy06" -- ∞  - 109
--- #gadget_display with_axioms "tim_easy07" -- 8  - 5
--- #gadget_display with_axioms "tim_easy08" -- ∞  - 42 - 15 | 36
--- #gadget_display with_axioms "tim_easy09" -- ∞  - 29 - ∞ - 34 - 36 - 34 | 40
--- #gadget_display with_axioms "tim_easy10" -- 14 - 8  - 5
--- #gadget_display with_axioms "tim_easy11" -- 3
--- #gadget_display with_axioms "tim_easy12" -- ∞  - 24 - 21 - 31 - 21 - 25 - 21 | 28
--- #gadget_display with_axioms "tim_easy13" -- 5  - 4
+#gadget_display with_axioms "tim_easy01" -- 6  - 5
+#gadget_display with_axioms "tim_easy02" -- 40 - 29 | 32
+#gadget_display with_axioms "tim_easy03" -- 40 - 11 - 13 - 5
+#gadget_display with_axioms "tim_easy04" -- ∞  - 10 - 11
+#gadget_display with_axioms "tim_easy05" -- ∞  - 59
+#gadget_display with_axioms "tim_easy06" -- ∞  - 109
+#gadget_display with_axioms "tim_easy07" -- 8  - 5
+#gadget_display with_axioms "tim_easy08" -- ∞  - 42 - 15 | 36
+#gadget_display with_axioms "tim_easy09" -- ∞  - 29 - ∞ - 34 - 36 - 34 | 40
+#gadget_display with_axioms "tim_easy10" -- 14 - 8  - 5
+#gadget_display with_axioms "tim_easy11" -- 3
+#gadget_display with_axioms "tim_easy12" -- ∞  - 24 - 21 - 31 - 21 - 25 - 21 | 28
+#gadget_display with_axioms "tim_easy13" -- 5  - 4
 
 -- #gadget_display with_axioms "jovan_easy02" -- 20
 
--- #gadget_display with_axioms "jacob25" 300
+-- #gadget_display with_axioms "tim44a"
 
-#exit
+-- #exit
 #gadget_display with_axioms "tim03" -- ∞ - 42
 #gadget_display with_axioms "tim04" -- 41 | 36
+#gadget_display with_axioms "tim05a" -- ∞ - 299
 #gadget_display with_axioms "tim07" -- ∞ - 267
 #gadget_display with_axioms "tim08" -- 24 | 28
 #gadget_display with_axioms "tim10" -- 23
 #gadget_display with_axioms "tim11" -- 13
-#gadget_display with_axioms "tim12" -- 213 | 307
-#gadget_display with_axioms "tim14" -- ∞ - 307
+-- #gadget_display with_axioms "tim12" -- 213 | 307
+#gadget_display with_axioms "tim14" -- ∞ - 39
 #gadget_display with_axioms "tim16" -- 17 | 19
 #gadget_display with_axioms "tim17" -- 28 | 9
 #gadget_display with_axioms "tim18" -- 19 | 18
 #gadget_display with_axioms "tim19" -- 12
 #gadget_display with_axioms "tim20" -- ∞ - 366
+#gadget_display with_axioms "tim22a" -- ∞ - 116
+#gadget_display with_axioms "tim22c" -- ∞ - 116
 #gadget_display with_axioms "tim23" -- 25
 #gadget_display with_axioms "tim24" -- 15 | 11
 #gadget_display with_axioms "tim25" -- 84 | 45
@@ -278,6 +281,7 @@ elab stx:"#gadget_display" axioms?:("with_axioms")? name:str timeout?:(num)? : c
 #gadget_display with_axioms "tim36" -- 12 | 15
 #gadget_display with_axioms "tim43" -- 11
 #gadget_display with_axioms "tim44" -- ∞ - 120
+#gadget_display with_axioms "tim44a" -- ∞ - 276
 #gadget_display with_axioms "tim46" -- 123 | 90
 
 /-
