web-proof-machine/GadgetGameSolver/GadgetGameSolver/Jovan/UnifySequence.lean
@@ -1,0 +1,446 @@
+import GadgetGameSolver.Jovan.Variables
+import GadgetGameSolver.Jovan.Util
+
+namespace JovanGadgetGame
+
+namespace Iterate
+
+structure MVarId where
+  id : Nat
+deriving Inhabited, BEq
+
+instance : Hashable MVarId where
+  hash mvarId := hash mvarId.id
+
+inductive Expr where
+| mvar : JovanGadgetGame.MVarId → Expr
+| imvar : MVarId → Int → Expr
+| app  : String → Array Expr → Expr
+deriving Inhabited, BEq
+
+structure Cell where
+  f    : String
+  args : Array Expr
+  deriving Inhabited
+
+def Expr.offsetByAux (e : Expr) (offset : Int) : Expr :=
+  match e with
+  | .imvar mvarId n => .imvar mvarId (n + offset)
+  | .app f args => .app f (args.attach.map fun ⟨arg, _⟩ => arg.offsetByAux offset)
+  | e => e
+
+def Expr.offsetBy (e : Expr) (offset : Int) : Expr :=
+  if offset == 0 then
+    e
+  else
+    e.offsetByAux offset
+
+end Iterate
+
+def AbstractedExpr.instantiateIterate (e : AbstractedExpr) (subst : Array Iterate.Expr) : Iterate.Expr :=
+  match e with
+  | .mvar i => subst[i]!
+  | .app f args => .app f <| args.attach.map fun ⟨arg, _⟩ => arg.instantiateIterate subst
+
+def AbstractedCell.instantiateIterate (c : AbstractedCell) (subst : Array Iterate.Expr) : Iterate.Cell where
+  f := c.f
+  args := c.args.map (·.instantiateIterate subst)
+
+namespace Iterate
+
+structure MVarDecl where
+  userName : String
+  deriving Inhabited
+
+inductive AssignmentKind where
+| noLoop : AssignmentKind
+| loop   : (up? root : Bool) → AssignmentKind
+deriving Inhabited
+
+@[inline]
+def AssignmentKind.isLoop : AssignmentKind → Bool
+| .noLoop   => false
+| .loop _ _ => true
+
+@[inline]
+def AssignmentKind.and (k k' : AssignmentKind) : Option AssignmentKind :=
+  match k, k' with
+  | .noLoop   , .noLoop    => some (.noLoop)
+  | .noLoop   , .loop up? _
+  | .loop up? _, .noLoop    => some (.loop up? false)
+  | .loop up? _, .loop up?' _ =>
+    if up? == up?' then some (.loop up? false) else none
+
+@[inline]
+def AssignmentKind.modify (k : AssignmentKind) (up? root : Bool) : Option AssignmentKind :=
+  match k with
+  | .noLoop => some (.loop up? root)
+  | .loop up?' _ => if up? == up?' then k else none
+
+/-- Structure for doing multiple `AssignmentKind.modify` operations at once. -/
+structure AssignmentKindModifier where
+  up   : Bool := false
+  down : Bool := false
+
+@[inline]
+def AssignmentKindModifier.insert (m : AssignmentKindModifier) (up? : Bool) : AssignmentKindModifier :=
+  if up? then
+    { m with up := true }
+  else
+    { m with down := true}
+
+@[inline]
+def AssignmentKindModifier.apply (m : AssignmentKindModifier) (up? isRoot : Bool) : Option AssignmentKind :=
+    if up? then
+      if m.down then none else some (.loop up? isRoot)
+    else
+      if m.up   then none else some (.loop up? isRoot)
+
+/-- Represents an assignment `aₙ₊ᵢ := value₊ᵢ` for all `i ∈ ℕ`. -/
+structure MVarAssignment where
+  n       : Int
+  value   : Expr
+  kind    : AssignmentKind
+  deriving Inhabited
+
+/-- Represents an assignment `mvarIdᵢ₊ₙ := value` for all `i ∈ ℕ`. -/
+structure PendingAssignment where
+  mvarId : MVarId
+  n      : Int
+  value  : Expr
+  deriving Inhabited
+
+structure MVarContext where
+  decls       : Std.HashMap MVarId MVarDecl       := {}
+  assignments : Std.HashMap MVarId MVarAssignment := {}
+  /-- `pending` contains unhandled assignments of loopy metavariables.
+  It should be empty at the start and end of unification. -/
+  pending     : Array PendingAssignment           := #[]
+  deriving Inhabited
+
+class MonadMCtx (m : Type → Type) where
+  getMCtx    : m MVarContext
+  modifyMCtx : (MVarContext → MVarContext) → m Unit
+
+export MonadMCtx (getMCtx modifyMCtx)
+
+instance (m) [MonadStateOf MVarContext m] : MonadMCtx m where
+  getMCtx    := get
+  modifyMCtx := modify
+
+@[always_inline]
+instance (m n) [MonadLift m n] [MonadMCtx m] : MonadMCtx n where
+  getMCtx      := liftM (getMCtx : m _)
+  modifyMCtx f := liftM (modifyMCtx f : m _)
+
+section
+
+variable {m : Type → Type} [Monad m] [MonadMCtx m] [MonadUnique m]
+
+@[inline] def setMCtx (mctx : MVarContext) : m Unit :=
+  modifyMCtx (fun _ => mctx)
+
+def mkFreshMVar (userName : String) : m Expr := do
+  let mvarId := { id := ← getUnique }
+  modifyMCtx fun mctx => { mctx with decls := mctx.decls.insert mvarId { userName } }
+  return .imvar mvarId 0
+
+def MVarId.getDecl! (mvarId : MVarId) : m MVarDecl := do
+  return (← getMCtx).decls[mvarId]!
+
+def MVarId.assign (mvarId : MVarId) (n : Int) (value : Expr) (kind : AssignmentKind) : m Unit :=
+  modifyMCtx fun mctx => { mctx with assignments := mctx.assignments.insert mvarId { n, value, kind } }
+
+def MVarId.getAssignment? (mvarId : MVarId) : m (Option MVarAssignment) := do
+  return (← getMCtx).assignments[mvarId]?
+
+@[inline]
+def pushPending (mvarId : MVarId) (n : Int) (value : Expr) : m Unit :=
+  modifyMCtx fun mctx => { mctx with pending := mctx.pending.push { mvarId, n, value } }
+
+end
+
+
+/-!
+
+
+* a₀ := f b₀
+* a₀ := f f a₁ =>
+  - merge `f b₀` and `f f a₁`
+  - a₀ := b₀
+  - b₀ := f a₁ (loop)
+
+In this example, the occurs check for `b₀` would ideally already know that `a₀ := b₀`.
+So, when assigning unassigned metavariables, we should delay this at all times.
+
+----
+
+To know the exact goals that come out of the unification sequence, we have to keep track of
+the boundary conditions on both end of the finite unification sequence.
+
+We can either do it the lazy way which is to take the smallest possible interval,
+or the hard way, which is to keep track of unions of intervals.
+
+Either way, we need a data structure called `Support`, which has a union and intersection operation.
+
+Then every variable assignment must have a `Support`, and the unification as a whole must have a `Support`.
+
+
+Let's try to see how to work with `Support`.
+
+A₁ =?= f (f A₀) (we can shift the indices freely in order to put store assignments at the 0-index)
+  assign A₀ := f (f A₋₁) `has to hold from n+1, where n is the first value at which unification succeeds`
+B₁ =?= f (f B₀)
+  assign B₀ := f (f B₋₁) `has to hold from n+1`
+A₁ =?= f B₀
+  try to assign A₀ := f B₋₁, `has to hold from n+1`
+  merge assignments f B₋₁ and f (f A₋₁) of A₀
+    in this merge, we don't instantiate B₋₁ because it has a loopy assignment
+  result of merge: f B₋₁, under condition that B₀ := f A₀
+    assign A₀ := f B₋₁ `Has to hold from n+1`
+    try to assign B₀ := f A₀ `Has to hold from n`
+    merge assignments f A₀ and f (f B₋₁) of B₀
+      in this merge, we don't instantiate A₀ because it has a loopy assignment
+    result of merge: f A₀, under condition that A₀ := f B₋₁
+      assign B₀ := f A₀ `Has to hold from n`
+      try to assign A₀ := f B₋₁ `Has to hold from n+1`
+      this assignment agrees with the assignment of A₀ that we have.
+
+In this example, we see that the unification simply works from the start (n = 0)
+We note that during merging, the merged result has to hold on the union,
+whereas the induced assignments have to hold on the intersection.
+  FALSE! how the induced assignments hold depends on which side we're assigning:
+    it inherits the support from the side it is being assigned to.
+    because if always x := f f z, and sometimes x := f y, and we set x := f y,
+    then we always need to have that f := f z.
+
+However, we should take care with unions if we case about finite unification results:
+The union of two intervals isn't the min/max of the start/end points.
+
+this one also just holds
+
+* a₀ := f f f f f a₅ `has to hold from n+x` [0, n-5]
+* a₀ := f f f a₃ `has to hold from n+y` [0, n-3]
+  - merge assignments `f f f a₃` and `f f f f f a₅`
+  - a₀ := f f f a₃ `has to hold from n+min(x, y)` [0, n-3]
+  - a₀ := f f a₂ ? `has to hold from n+x+3` [3, n-2]
+    - merge assignments `f f a₂` and `f f f a₃`
+    - a₀ := f f a₂ `has to hold from n+min(x, y)` [0, n-3]∪[3, n-2]
+    - a₀ := f a₁ ? `has to hold from n+2+min(x, y)` [2, n-1]
+      - merge assignments `f a₁` and `f f a₂`
+      - a₀ := f a₁ `has to hold from n+min(x, y)` [0, n-3]∪[2, n-1]
+      - a₀ := f a₁ ? `has to hold from n+1+min(x, y)` [0, n-3]∪[3, n-2]
+        - merge assignments `f a₁` and `f a₁`
+        - a₀ := f a₁ `has to hold from n+min(x, y)` [0, n-3]∪[2, n-1]
+        - a₀ := a₀ `has to hold from n+1+min(x, y)`
+
+
+example where the forced assignments require involvement of negative variables:
+
+* a₀ := b₋₁ `has to hold from n+1`
+* b₀ := c₋₁ `has to hold from n+1`
+* c₀ := d₋₁ `has to hold from n+1`
+* d₀ := e₋₁ `has to hold from n+1`
+NOTICE: writing these assignments the other way around is much more favourable.
+
+Then when we instantiate metavariables we notice that the supports aren't good enought for our purpose.
+So we may expand the supports to force our equation to be satisfied.
+Or we may accept the lack of support and update the unification that we're making work.
+
+The problem with expanding the supports is that we also involve metavariables that we don't want to exist.
+Better would be to only involve the legal metavariables from the start.
+So while instantiating metavariables, we keep track of the support, realizing that we can't support
+certain assignments anymore.
+
+What about this
+
+* a₀ := b₋₁ `has to hold from n+1`
+* b₀ := c₀ `has to hold from n+1`
+
+The we force the assignment of `b₀ := c₀` to also hold at 0. But that doesn't mean that
+any illegal metavariables have been added.
+Whereas the method of accepting lack of support is going to behave badly here.
+
+
+-/
+
+abbrev M := EStateM Unit MVarContext
+
+instance : Alternative M where
+  failure := throw ()
+  orElse  := tryCatch
+
+private structure OccursContext where
+  mvarId  : MVarId
+  offset  : Int -- how much we should subtract from the expression
+  mvarIds : List MVarId := []
+  kindMod : AssignmentKindModifier := {}
+
+@[inline]
+private def OccursContext.insert (mvarId : MVarId) (up? : Bool) (c : OccursContext) : OccursContext :=
+  { c with mvarIds := mvarId :: c.mvarIds, kindMod := c.kindMod.insert up? }
+
+/-
+Fails inside `M` if occurs check failed. Fails inside `OptionT` if it failed at the root.
+If other variables become loopy due to this assignment, we store that.
+-/
+partial def Expr.occursCheck (context : OccursContext) (isRoot : Bool) : Expr → M (Option AssignmentKind)
+  | .imvar mvarId n' => do
+    if mvarId == context.mvarId then
+      match compare n' context.offset with
+      | .lt => return context.kindMod.apply false isRoot
+      | .eq => return none
+      | .gt => return context.kindMod.apply true  isRoot
+    else
+      let some { n, value, kind } ← mvarId.getAssignment? | return some .noLoop
+      let context := { context with offset := context.offset + n - n' }
+      match kind with
+      | .noLoop =>
+        let some kind ← value.occursCheck context isRoot | return none
+        /- We make sure variables part of a new loop are set to loopy. -/
+        if kind.isLoop then
+          mvarId.assign n value kind
+        return kind
+      | .loop up? _ =>
+        if context.mvarIds.contains mvarId then
+          return some .noLoop
+        else
+          value.occursCheck (context.insert mvarId up?) isRoot
+  | .app _ args =>
+    some <$> args.foldlM (init := .noLoop) fun result arg => do
+      let some kind ← arg.occursCheck context false | failure
+      (result.and kind).getM
+  | .mvar _ => return some .noLoop
+
+
+
+/--
+Merges assignments `aᵢ := s` and `aⱼ := t` for `i ≤ j`. We have `offset := i - j`.
+
+Computes the common part of two expressions, leaving the metavariables that were at the leaves.
+The required metavariable assignments are added as `PendingAssignments` in the context.
+-/
+private partial def mergeCore (s t : Expr) (offset : Int) : M Expr := do
+  let returnMVar mvarId n t := do
+    pushPending mvarId n t
+    return .imvar mvarId n
+
+  match s, t with
+  | .imvar mvarId n, .imvar mvarId' n' =>
+    let n' := n' + offset
+    /- This case split is crucial for termination of the algorithm, as it reduces
+      the index offset at mvar-to-mvar assignments. -/
+    match compare n n' with
+    | .lt => returnMVar mvarId' n' s
+    | .eq =>
+      if mvarId == mvarId' then return s
+      else returnMVar mvarId' n' s
+    | .gt =>
+      returnMVar mvarId n (.imvar mvarId' n')
+  | .imvar mvarId n, t   => returnMVar mvarId n (t.offsetBy offset)
+  | s, .imvar mvarId' n' => returnMVar mvarId' (n' + offset) s
+  | .app f args, .app f' args' => do
+    if h : f = f' ∧ args.size = args'.size then
+      let args ← args.size.foldM' (init := .mkEmpty args.size) fun i mergeArgs =>
+        mergeArgs.push <$> mergeCore args[i] args'[i] offset
+      return .app f args
+    else
+      failure
+  | .mvar mvarId, .mvar mvarId' => if mvarId == mvarId' then return s else failure
+  | _, _ => failure
+
+private partial def instantiateRootLoop (startMvarId mvarId : MVarId) (startN n : Int) : M Int := do
+  if mvarId == startMvarId then
+    assert! n < startN
+    return startN - n
+  else
+    let some { n := assigN, value := .imvar mvarId' assigN', kind } ← mvarId.getAssignment? | unreachable!
+    let n' := n + assigN' - assigN
+    if assigN > n then
+      mvarId.assign assigN (.imvar mvarId' n') kind
+    instantiateRootLoop startMvarId mvarId' startN n'
+
+/--
+`mergeCore` jumps throught some hoops in order to ensure the algorithm terminates.
+-/
+def merge (s t : Expr) (sKind tKind : AssignmentKind) (ns nt : Int) (mvarId : MVarId) : M Expr := do
+  match sKind, tKind with
+  | .loop _ true, .loop _ true => mergeCore s t (ns - nt)
+  | .loop _ true, _ =>
+    let .imvar mvarId' n' := s | unreachable!
+    let period ← instantiateRootLoop mvarId mvarId' ns n'
+    mergeCore (t.offsetBy period) t period
+  | _, .loop _ true =>
+    let .imvar mvarId' n' := t | unreachable!
+    let period ← instantiateRootLoop mvarId mvarId' nt n'
+    mergeCore (s.offsetBy period) s period
+  | _, _ =>
+    mergeCore s t (ns - nt)
+
+partial def processPending : M Unit := do
+  let { pending, .. } ← getMCtx
+  if pending.isEmpty then
+    return
+  else
+    let { mvarId, n := nNew, value := newValue } := pending.back
+    modifyMCtx ({ · with pending := pending.pop })
+    let some newKind ← newValue.occursCheck { mvarId, offset := nNew } true | return -- `value = .imvar mvarId nNew`
+    match ← mvarId.getAssignment? with
+    | some { n, value, kind } =>
+      -- we assign at the smallest value of `n`. This can create too strong assignments, but that's acceptable.
+      if nNew < n then
+        let value ← merge newValue value newKind kind nNew n mvarId
+        mvarId.assign nNew value kind
+      else
+        let value ← merge value newValue kind newKind n nNew mvarId
+        mvarId.assign n value kind
+    | none =>
+      mvarId.assign nNew newValue newKind
+
+    processPending
+
+
+partial def unifyCore (s t : Expr) : M Unit := do
+  match s, t with
+  | .imvar mvarId n, .imvar mvarId' n' =>
+    match compare n n' with
+    | .lt => pushPending mvarId' n' s
+    | .eq =>
+      if mvarId == mvarId' then return
+      else pushPending mvarId' n' s
+    | .gt =>
+      pushPending mvarId n (.imvar mvarId' n')
+  | .imvar mvarId n, t   => pushPending mvarId  n  t
+  | s, .imvar mvarId' n' => pushPending mvarId' n' s
+  | .app f args, .app f' args' => do
+    if h : f = f' ∧ args.size = args'.size then
+      args.size.forM' fun i =>
+        unifyCore args[i] args'[i]
+    else
+      failure
+  | .mvar mvarId, .mvar mvarId' => if mvarId == mvarId' then return else failure
+  | _, _ => failure
+
+
+def unify (s t : Expr) : Option MVarContext := do
+  match unifyCore s t |>.run {} with
+  | .ok () ctx  => some ctx
+  | .error () _ => none
+
+
+end Iterate
+
+/-
+
+Would it make sense to use a e-graph like data structure for my infinite unifications?
+
+* Term graph: all terms, represented in a way to maximize sharing.
+
+* Union-find: all equivalences on the terms.
+
+Now, the only terms that should be allowed in the union-find are variable assignments,
+and the congruences created from them, from the
+
+
+
+-/
